Fix old fstart code.
Signed-off-by: Aliwoto <aminnimaj@gmail.com>

basic_proofs/FunctionSurjectivity.fst
@@ -6,13 +6,13 @@ module FunctionSurjectivity
 type even_int = n:int{n % 2 == 0}
 
 (* Our function: double any integer *)
-let double (x:int) : even_int = (op_Multiply 2 x)
+let double (x:int) : even_int = 2 * x
 
 (* Witness function: for any even integer, find a pre-image *)
 let half (e:even_int) : int = (e / 2)
 
 (* Custom lemma: For even integers e, 2 * (e / 2) = e *)
-let lemma_double_half_even (e:even_int) : Lemma (ensures (op_Multiply 2 (e / 2)) == e) =
+let lemma_double_half_even (e:even_int) : Lemma (ensures (2 * (e / 2)) == e) =
   // For even integers e, e % 2 = 0
   // By Euclidean division: e = (e / 2) * 2 + (e % 2)
   // Since e % 2 = 0, we have e = (e / 2) * 2
@@ -25,7 +25,7 @@ let double_surjective() : Lemma (forall (e:even_int). double (half e) == e) =
     calc (==) {
       double (half e);
       == {}
-      op_Multiply 2 (e / 2);
+      2 * (e / 2);
       == { lemma_double_half_even e }
       e;
     }
