basic_proofs/AbsorptionLaws.fst
@@ -2,7 +2,7 @@ module AbsorptionLaws
 
 // Lemma for the first Absorption Law: p \/ (p /\ q) <==> p
 
-val absorption_law_1 (p q: Type0) : Lemma ((p \/ (p /\ q)) <==> p)
+val absorption_law_1 (p q: prop) : Lemma ((p \/ (p /\ q)) <==> p)
 
 let absorption_law_1 p q = () // Proof is automatic for this basic tautology
 
@@ -14,9 +14,9 @@ let absorption_law_1 p q = () // Proof is automatic for this basic tautology
 // The <==> operator is a binary logical operator that takes two propositions on 
 // its left and right sides and forms a new proposition which is true if and only if
 // both sides have the same truth value.
-let absorption_law1_intermediate (p q r: Type0) = ((p \/ p) /\ (p \/ q) /\ (p \/ r))
+let absorption_law1_intermediate (p q r: prop) = ((p \/ p) /\ (p \/ q) /\ (p \/ r))
 
-val absorption_law1_v2 (p q r: Type0)
+val absorption_law1_v2 (p q r: prop)
     : Lemma
     (((p \/ (p /\ q /\ r)) <==> absorption_law1_intermediate p q r) /\
       (absorption_law1_intermediate p q r <==> p))
@@ -25,7 +25,7 @@ let absorption_law1_v2 p q r = ()
 
 // Lemma for the second Absorption Law: p /\ (p \/ q) <==> p
 
-val absorption_law_2 (p q: Type0) : Lemma ((p /\ (p \/ q)) <==> p)
+val absorption_law_2 (p q: prop) : Lemma ((p /\ (p \/ q)) <==> p)
 
 let absorption_law_2 p q = () // Proof is automatic for this basic tautology
 
