basic_proofs/ContrapositionLaws.fst
@@ -3,6 +3,6 @@ module ContrapositionLaws
 // Let P and Q be two propositions.
 // (P ⟹ Q) ⟺ (¬Q ⟹ ¬P)
 
-let contraposition (p: Type0) (q: Type0) : Lemma 
+let contraposition (p: prop) (q: prop) : Lemma 
   (ensures (p ==> q) <==> (~q ==> ~p)) = 
   ()
