basic_proofs/TransitivityLaws.fst
@@ -1,6 +1,6 @@
 module TransitivityLaws
 
-let transitive_implication (p q r : Type0) : Lemma
+let transitive_implication (p q r : prop) : Lemma
   (requires (p ==> q) /\ (q ==> r))
   (ensures (p ==> r))
   = ()
